examples/miniML/compiler/correctness/miscScript.sml
@@ -1,0 +1,536 @@
+open HolKernel bossLib boolLib boolSimps listTheory pred_setTheory finite_mapTheory alistTheory lcsymtacs
+val _ = new_theory "misc"
+
+(* Misc. lemmas (without any compiler constants) *)
+
+(* TODO: move *)
+val cond_sum_expand = store_thm(
+"cond_sum_expand",
+``(!x y z. ((if P then INR x else INL y) = INR z) = (P /\ (z = x))) /\
+  (!x y z. ((if P then INR x else INL y) = INL z) = (~P /\ (z = y))) /\
+  (!x y z. ((if P then INL x else INR y) = INL z) = (P /\ (z = x))) /\
+  (!x y z. ((if P then INL x else INR y) = INR z) = (~P /\ (z = y)))``,
+Cases_on `P` >> fs[] >> rw[EQ_IMP_THM])
+
+val FOLDR_CONS_triple = store_thm(
+"FOLDR_CONS_triple",
+``!f ls a. FOLDR (\(x,y,z) w. f x y z :: w) a ls = (MAP (\(x,y,z). f x y z) ls)++a``,
+GEN_TAC THEN
+Induct THEN1 SRW_TAC[][] THEN
+Q.X_GEN_TAC `p` THEN
+PairCases_on `p` THEN
+SRW_TAC[][])
+
+val FOLDL2_FUPDATE_LIST = store_thm(
+"FOLDL2_FUPDATE_LIST",
+``!f1 f2 bs cs a. (LENGTH bs = LENGTH cs) ⇒
+  (FOLDL2 (λfm b c. fm |+ (f1 b c, f2 b c)) a bs cs =
+   a |++ ZIP (MAP2 f1 bs cs, MAP2 f2 bs cs))``,
+SRW_TAC[][FUPDATE_LIST,FOLDL2_FOLDL,MAP2_MAP,ZIP_MAP,MAP_ZIP,
+          rich_listTheory.FOLDL_MAP,rich_listTheory.LENGTH_MAP2,
+          LENGTH_ZIP,pairTheory.LAMBDA_PROD])
+
+val FOLDL2_FUPDATE_LIST_paired = store_thm(
+"FOLDL2_FUPDATE_LIST_paired",
+``!f1 f2 bs cs a. (LENGTH bs = LENGTH cs) ⇒
+  (FOLDL2 (λfm b (c,d). fm |+ (f1 b c d, f2 b c d)) a bs cs =
+   a |++ ZIP (MAP2 (λb. UNCURRY (f1 b)) bs cs, MAP2 (λb. UNCURRY (f2 b)) bs cs))``,
+rw[FOLDL2_FOLDL,MAP2_MAP,ZIP_MAP,MAP_ZIP,LENGTH_ZIP,
+   pairTheory.UNCURRY,pairTheory.LAMBDA_PROD,FUPDATE_LIST,
+   rich_listTheory.FOLDL_MAP])
+
+val FOLDL_FUPDATE_LIST = store_thm(
+"FOLDL_FUPDATE_LIST",
+``!f1 f2 ls a. FOLDL (\fm k. fm |+ (f1 k, f2 k)) a ls =
+  a |++ MAP (\k. (f1 k, f2 k)) ls``,
+SRW_TAC[][FUPDATE_LIST,rich_listTheory.FOLDL_MAP])
+
+val FUN_FMAP_FAPPLY_FEMPTY_FAPPLY = store_thm(
+"FUN_FMAP_FAPPLY_FEMPTY_FAPPLY",
+``FINITE s ==> (FUN_FMAP ($FAPPLY FEMPTY) s ' x = FEMPTY ' x)``,
+Cases_on `x IN s` >>
+rw[FUN_FMAP_DEF,NOT_FDOM_FAPPLY_FEMPTY])
+val _ = export_rewrites["FUN_FMAP_FAPPLY_FEMPTY_FAPPLY"]
+
+val FUPDATE_LIST_APPLY_NOT_MEM_matchable = store_thm(
+"FUPDATE_LIST_APPLY_NOT_MEM_matchable",
+``!kvl f k v. ~MEM k (MAP FST kvl) /\ (v = f ' k) ==> ((f |++ kvl) ' k = v)``,
+PROVE_TAC[FUPDATE_LIST_APPLY_NOT_MEM])
+
+val FST_triple = store_thm(
+"FST_triple",
+``(λ(n,ns,b). n) = FST``,
+rw[FUN_EQ_THM,pairTheory.UNCURRY])
+
+val SND_triple = store_thm(
+"SND_triple",
+``(λ(n,ns,b). f ns b) = UNCURRY f o SND``,
+rw[FUN_EQ_THM,pairTheory.UNCURRY])
+
+val FST_pair = store_thm(
+"FST_pair",
+``(λ(n,v). n) = FST``,
+rw[FUN_EQ_THM,pairTheory.UNCURRY])
+
+val SND_pair = store_thm(
+"SND_pair",
+``(λ(n,v). v) = SND``,
+rw[FUN_EQ_THM,pairTheory.UNCURRY])
+
+val SND_FST_pair = store_thm(
+"SND_FST_pair",
+``(λ((n,m),c).m) = SND o FST``,
+rw[FUN_EQ_THM,pairTheory.UNCURRY])
+
+val set_MAP_FST_fmap_to_alist = store_thm(
+"set_MAP_FST_fmap_to_alist",
+``set (MAP FST (fmap_to_alist fm)) = FDOM fm``,
+METIS_TAC[fmap_to_alist_to_fmap,FDOM_alist_to_fmap])
+val _ = export_rewrites["set_MAP_FST_fmap_to_alist"]
+
+val DIFF_UNION = store_thm(
+"DIFF_UNION",
+``!x y z. x DIFF (y UNION z) = x DIFF y DIFF z``,
+SRW_TAC[][EXTENSION] THEN METIS_TAC[])
+
+val DIFF_COMM = store_thm(
+"DIFF_COMM",
+``!x y z. x DIFF y DIFF z = x DIFF z DIFF y``,
+SRW_TAC[][EXTENSION] THEN METIS_TAC[])
+
+val INJ_I = store_thm(
+"INJ_I",
+``∀s t. INJ I s t = s ⊆ t``,
+SRW_TAC[][INJ_DEF,SUBSET_DEF])
+
+val MAP_KEYS_I = store_thm(
+"MAP_KEYS_I",
+``∀fm. MAP_KEYS I fm = fm``,
+rw[GSYM fmap_EQ_THM,MAP_KEYS_def,EXTENSION] >>
+metis_tac[MAP_KEYS_def,INJ_I,SUBSET_UNIV,combinTheory.I_THM])
+val _ = export_rewrites["MAP_KEYS_I"]
+
+val MAP_EQ_ID = store_thm(
+"MAP_EQ_ID",
+``!f ls. (MAP f ls = ls) = (!x. MEM x ls ==> (f x = x))``,
+PROVE_TAC[MAP_EQ_f,MAP_ID,combinTheory.I_THM])
+
+(* TODO: move *)
+val LIST_REL_EVERY_ZIP = store_thm(
+"LIST_REL_EVERY_ZIP",
+``!R l1 l2. LIST_REL R l1 l2 = ((LENGTH l1 = LENGTH l2) /\ EVERY (UNCURRY R) (ZIP (l1,l2)))``,
+GEN_TAC THEN Induct THEN SRW_TAC[][LENGTH_NIL_SYM] THEN
+SRW_TAC[][EQ_IMP_THM,LIST_REL_CONS1] THEN SRW_TAC[][] THEN
+Cases_on `l2` THEN FULL_SIMP_TAC(srw_ss())[])
+
+val MAP_ZIP_SND_triple = store_thm(
+"MAP_ZIP_SND_triple",
+``(LENGTH l1 = LENGTH l2) ⇒ (MAP (λ(x,y,z). f y z) (ZIP(l1,l2)) = MAP (UNCURRY f) l2)``,
+strip_tac >> (
+MAP_ZIP
+|> Q.GEN`g`
+|> Q.ISPEC `UNCURRY (f:'b->'c->'d)`
+|> SIMP_RULE(srw_ss())[combinTheory.o_DEF,pairTheory.LAMBDA_PROD]
+|> UNDISCH_ALL
+|> CONJUNCTS
+|> Lib.el 4
+|> MATCH_ACCEPT_TAC))
+
+val FUPDATE_LIST_APPLY_HO_THM = store_thm(
+"FUPDATE_LIST_APPLY_HO_THM",
+``∀P f kvl k.
+(∃n. n < LENGTH kvl ∧ (k = EL n (MAP FST kvl)) ∧ P (EL n (MAP SND kvl)) ∧
+     (∀m. n < m ∧ m < LENGTH kvl ⇒ EL m (MAP FST kvl) ≠ k)) ∨
+(¬MEM k (MAP FST kvl) ∧ P (f ' k))
+⇒ (P ((f |++ kvl) ' k))``,
+metis_tac[FUPDATE_LIST_APPLY_MEM,FUPDATE_LIST_APPLY_NOT_MEM])
+
+val LESS_1 = store_thm(
+"LESS_1",
+``x < 1 = (x = 0:num)``,
+DECIDE_TAC)
+val _ = export_rewrites["LESS_1"]
+
+val FRANGE_FUPDATE_LIST_SUBSET = store_thm(
+"FRANGE_FUPDATE_LIST_SUBSET",
+``∀ls fm. FRANGE (fm |++ ls) ⊆ FRANGE fm ∪ (set (MAP SND ls))``,
+Induct >- rw[FUPDATE_LIST_THM] >>
+qx_gen_tac `p` >> qx_gen_tac `fm` >>
+pop_assum (qspec_then `fm |+ p` mp_tac) >>
+srw_tac[DNF_ss][SUBSET_DEF] >>
+first_x_assum (qspec_then `x` mp_tac) >> fs[FUPDATE_LIST_THM] >>
+rw[] >> fs[] >>
+PairCases_on `p` >>
+fsrw_tac[DNF_ss][FRANGE_FLOOKUP,FLOOKUP_UPDATE] >>
+pop_assum mp_tac >> rw[] >>
+PROVE_TAC[])
+
+val IN_FRANGE_FUPDATE_LIST_suff = store_thm(
+"IN_FRANGE_FUPDATE_LIST_suff",
+``(∀v. v ∈ FRANGE fm ⇒ P v) ∧ (∀v. MEM v (MAP SND ls) ⇒ P v) ⇒
+    ∀v. v ∈ FRANGE (fm |++ ls) ⇒ P v``,
+rw[] >>
+imp_res_tac(SIMP_RULE(srw_ss())[SUBSET_DEF]FRANGE_FUPDATE_LIST_SUBSET) >>
+PROVE_TAC[])
+
+(* TODO: move *)
+val IN_FRANGE = store_thm(
+"IN_FRANGE",
+``!f v. v IN FRANGE f = ?k. k IN FDOM f /\ (f ' k = v)``,
+SRW_TAC[][FRANGE_DEF])
+
+val FRANGE_FUNION_SUBSET = store_thm(
+"FRANGE_FUNION_SUBSET",
+``FRANGE (f1 ⊌ f2) ⊆ FRANGE f1 ∪ FRANGE f2``,
+srw_tac[DNF_ss][FRANGE_DEF,SUBSET_DEF,FUNION_DEF] >>
+PROVE_TAC[])
+
+val FRANGE_DOMSUB_SUBSET = store_thm(
+"FRANGE_DOMSUB_SUBSET",
+``FRANGE (fm \\ k) ⊆ FRANGE fm``,
+srw_tac[DNF_ss][FRANGE_DEF,SUBSET_DEF,DOMSUB_FAPPLY_THM] >>
+PROVE_TAC[])
+
+val FRANGE_DRESTRICT_SUBSET = store_thm(
+"FRANGE_DRESTRICT_SUBSET",
+``FRANGE (DRESTRICT fm s) ⊆ FRANGE fm``,
+srw_tac[DNF_ss][FRANGE_DEF,SUBSET_DEF,DRESTRICT_DEF] >>
+PROVE_TAC[])
+
+val IN_FRANGE_FUNION_suff = store_thm(
+"IN_FRANGE_FUNION_suff",
+``(∀v. v ∈ FRANGE f1 ⇒ P v) ∧ (∀v. v ∈ FRANGE f2 ⇒ P v) ⇒
+  (∀v. v ∈ FRANGE (f1 ⊌ f2) ⇒ P v)``,
+rw[] >>
+imp_res_tac(SIMP_RULE(srw_ss())[SUBSET_DEF]FRANGE_FUNION_SUBSET) >>
+PROVE_TAC[])
+
+val IN_FRANGE_DOMSUB_suff = store_thm(
+"IN_FRANGE_DOMSUB_suff",
+``(∀v. v ∈ FRANGE fm ⇒ P v) ⇒ (∀v. v ∈ FRANGE (fm \\ k) ⇒ P v)``,
+rw[] >>
+imp_res_tac(SIMP_RULE(srw_ss())[SUBSET_DEF]FRANGE_DOMSUB_SUBSET) >>
+PROVE_TAC[])
+
+val IN_FRANGE_DRESTRICT_suff = store_thm(
+"IN_FRANGE_DRESTRICT_suff",
+``(∀v. v ∈ FRANGE fm ⇒ P v) ⇒ (∀v. v ∈ FRANGE (DRESTRICT fm s) ⇒ P v)``,
+rw[] >>
+imp_res_tac(SIMP_RULE(srw_ss())[SUBSET_DEF]FRANGE_DRESTRICT_SUBSET) >>
+PROVE_TAC[])
+
+val exists_list_GENLIST = store_thm(
+"exists_list_GENLIST",
+``(∃ls. P ls) = (∃n f. P (GENLIST f n))``,
+rw[EQ_IMP_THM] >- (
+  map_every qexists_tac [`LENGTH ls`,`combin$C EL ls`] >>
+  qmatch_abbrev_tac `P ls2` >>
+  qsuff_tac `ls2 = ls` >- rw[] >>
+  rw[LIST_EQ_REWRITE,Abbr`ls2`] ) >>
+PROVE_TAC[])
+
+val DRESTRICT_SUBMAP_gen = store_thm(
+"DRESTRICT_SUBMAP_gen",
+``f SUBMAP g ==> DRESTRICT f P SUBMAP g``,
+SRW_TAC[][SUBMAP_DEF,DRESTRICT_DEF])
+
+val DRESTRICT_SUBSET_SUBMAP = store_thm(
+"DRESTRICT_SUBSET_SUBMAP",
+``s1 SUBSET s2 ==> DRESTRICT f s1 SUBMAP DRESTRICT f s2``,
+SRW_TAC[][SUBMAP_DEF,SUBSET_DEF,DRESTRICT_DEF])
+
+val FUPDATE_SAME_APPLY = store_thm(
+"FUPDATE_SAME_APPLY",
+``(x = FST kv) \/ (fm1 ' x = fm2 ' x) ==> ((fm1 |+ kv) ' x = (fm2 |+ kv) ' x)``,
+Cases_on `kv` >> rw[FAPPLY_FUPDATE_THM])
+
+val FUPDATE_SAME_LIST_APPLY = store_thm(
+"FUPDATE_SAME_LIST_APPLY",
+``!kvl fm1 fm2 x. MEM x (MAP FST kvl) ==> ((fm1 |++ kvl) ' x = (fm2 |++ kvl) ' x)``,
+ho_match_mp_tac SNOC_INDUCT >>
+conj_tac >- rw[] >>
+rw[FUPDATE_LIST,FOLDL_SNOC] >>
+match_mp_tac FUPDATE_SAME_APPLY >>
+qmatch_rename_tac `(y = FST p) \/ Z` ["Z"] >>
+Cases_on `y = FST p` >> rw[] >>
+first_x_assum match_mp_tac >>
+fs[MEM_MAP] >>
+PROVE_TAC[])
+
+val DRESTRICTED_FUNION = store_thm(
+"DRESTRICTED_FUNION",
+``∀f1 f2 s. DRESTRICT (f1 ⊌ f2) s = DRESTRICT f1 s ⊌ DRESTRICT f2 (s DIFF FDOM f1)``,
+rw[GSYM fmap_EQ_THM,DRESTRICT_DEF,FUNION_DEF] >> rw[] >>
+rw[EXTENSION] >> PROVE_TAC[])
+
+(* TODO: move *)
+val OPTREL_refl = store_thm(
+"OPTREL_refl",
+``(!x. R x x) ==> !x. OPTREL R x x``,
+strip_tac >> Cases >> rw[optionTheory.OPTREL_def])
+val _ = export_rewrites["OPTREL_refl"]
+
+(* TODO: move? *)
+val ALOOKUP_NONE = store_thm(
+"ALOOKUP_NONE",
+``!l x. (ALOOKUP l x = NONE) = ~MEM x (MAP FST l)``,
+SRW_TAC[][ALOOKUP_FAILS,MEM_MAP,pairTheory.FORALL_PROD])
+
+(* TODO: move? *)
+val DIFF_SAME_UNION = store_thm(
+"DIFF_SAME_UNION",
+``!x y. ((x UNION y) DIFF x = y DIFF x) /\ ((x UNION y) DIFF y = x DIFF y)``,
+SRW_TAC[][EXTENSION,EQ_IMP_THM])
+
+val FOLDR_transitive_property = store_thm(
+"FOLDR_transitive_property",
+``!P ls f a. P [] a /\ (!n a. n < LENGTH ls /\ P (DROP (SUC n) ls) a ==> P (DROP n ls) (f (EL n ls) a)) ==> P ls (FOLDR f a ls)``,
+GEN_TAC THEN Induct THEN SRW_TAC[][] THEN
+`P ls (FOLDR f a ls)` by (
+  FIRST_X_ASSUM MATCH_MP_TAC THEN
+  SRW_TAC[][] THEN
+  Q.MATCH_ASSUM_RENAME_TAC `P (DROP (SUC n) ls) b` [] THEN
+  FIRST_X_ASSUM (Q.SPECL_THEN [`SUC n`,`b`] MP_TAC) THEN
+  SRW_TAC[][] ) THEN
+FIRST_X_ASSUM (Q.SPEC_THEN `0` MP_TAC) THEN
+SRW_TAC[][])
+
+val MEM_DROP = store_thm(
+"MEM_DROP",
+``!x ls n. MEM x (DROP n ls) = (n < LENGTH ls /\ (x = (EL n ls))) \/ MEM x (DROP (SUC n) ls)``,
+GEN_TAC THEN
+Induct THEN1 SRW_TAC[][] THEN
+NTAC 2 GEN_TAC THEN
+SIMP_TAC (srw_ss()) [] THEN
+Cases_on `n` THEN SIMP_TAC (srw_ss()) [] THEN
+PROVE_TAC[])
+
+(* TODO: Move *)
+val alist_to_fmap_PERM = store_thm(
+"alist_to_fmap_PERM",
+``∀l1 l2. PERM l1 l2 ∧ ALL_DISTINCT (MAP FST l1) ⇒ (alist_to_fmap l1 = alist_to_fmap l2)``,
+let open sortingTheory in
+qsuff_tac
+  `∀l1 l2. PERM l1 l2 ⇒ ALL_DISTINCT (MAP FST l1) ⇒ PERM l1 l2 ∧ (alist_to_fmap l1 = alist_to_fmap l2)`
+  >- rw[] >>
+ho_match_mp_tac PERM_IND >>
+fs[pairTheory.FORALL_PROD] >>
+rw[] >> fs[] >- (
+  fs[PERM_SWAP_AT_FRONT] )
+>- (
+  match_mp_tac FUPDATE_COMMUTES >> rw[] )
+>- (
+  PROVE_TAC[PERM_TRANS,ALL_DISTINCT_PERM,PERM_MAP] )
+>- (
+  PROVE_TAC[PERM_TRANS,ALL_DISTINCT_PERM,PERM_MAP] )
+end)
+
+(* TODO: move *)
+val DROP_APPEND1 = rich_listTheory.BUTFIRSTN_APPEND1
+val DROP_APPEND2 = rich_listTheory.BUTFIRSTN_APPEND2
+val DROP_LENGTH_NIL = rich_listTheory.BUTFIRSTN_LENGTH_NIL
+
+val MAP_values_fmap_to_alist = store_thm(
+"MAP_values_fmap_to_alist",
+``∀f fm. MAP (λ(k,v). (k, f v)) (fmap_to_alist fm) = fmap_to_alist (f o_f fm)``,
+rw[fmap_to_alist_def,MAP_MAP_o,MAP_EQ_f])
+
+val alist_to_fmap_MAP_matchable = store_thm(
+"alist_to_fmap_MAP_matchable",
+``∀f1 f2 al mal v. INJ f1 (set (MAP FST al)) UNIV ∧
+  (mal = MAP (λ(x,y). (f1 x,f2 y)) al) ∧
+  (v = MAP_KEYS f1 (f2 o_f alist_to_fmap al)) ⇒
+  (alist_to_fmap mal = v)``,
+METIS_TAC[alist_to_fmap_MAP])
+
+val alist_to_fmap_MAP_values = store_thm(
+"alist_to_fmap_MAP_values",
+``∀f al. alist_to_fmap (MAP (λ(k,v). (k, f v)) al) = f o_f (alist_to_fmap al)``,
+rw[] >>
+Q.ISPECL_THEN [`I:γ->γ`,`f`,`al`] match_mp_tac alist_to_fmap_MAP_matchable >>
+rw[INJ_I])
+
+val FRANGE_alist_to_fmap_SUBSET = store_thm(
+"FRANGE_alist_to_fmap_SUBSET",
+``FRANGE (alist_to_fmap ls) ⊆ IMAGE SND (set ls)``,
+srw_tac[DNF_ss][FRANGE_DEF,SUBSET_DEF,pairTheory.EXISTS_PROD] >>
+qmatch_assum_rename_tac `MEM z (MAP FST ls)`[] >>
+qexists_tac `z` >>
+match_mp_tac alist_to_fmap_FAPPLY_MEM >>
+rw[])
+
+val FRANGE_FUPDATE_SUBSET = store_thm(
+"FRANGE_FUPDATE_SUBSET",
+``FRANGE (fm |+ kv) ⊆ FRANGE fm ∪ {SND kv}``,
+Cases_on `kv` >>
+rw[FRANGE_DEF,SUBSET_DEF,DOMSUB_FAPPLY_THM] >>
+rw[] >> PROVE_TAC[])
+
+val IN_FRANGE_alist_to_fmap_suff = store_thm(
+"IN_FRANGE_alist_to_fmap_suff",
+``(∀v. MEM v (MAP SND ls) ⇒ P v) ⇒ (∀v. v ∈ FRANGE (alist_to_fmap ls) ⇒ P v)``,
+rw[] >>
+imp_res_tac(SIMP_RULE(srw_ss())[SUBSET_DEF]FRANGE_alist_to_fmap_SUBSET) >>
+fs[MEM_MAP] >>
+PROVE_TAC[])
+
+val IN_FRANGE_FUPDATE_suff = store_thm(
+"IN_FRANGE_FUPDATE_suff",
+`` (∀v. v ∈ FRANGE fm ⇒ P v) ∧ (P (SND kv))
+⇒ (∀v. v ∈ FRANGE (fm |+ kv) ⇒ P v)``,
+rw[] >>
+imp_res_tac(SIMP_RULE(srw_ss())[SUBSET_DEF]FRANGE_FUPDATE_SUBSET) >>
+fs[])
+
+val DRESTRICT_FDOM = store_thm(
+"DRESTRICT_FDOM",
+``!f.DRESTRICT f (FDOM f) = f``,
+SRW_TAC[][GSYM fmap_EQ_THM,DRESTRICT_DEF])
+
+(* TODO: move? *)
+val fmap_rel_def = Define`
+  fmap_rel R f1 f2 = (FDOM f2 = FDOM f1) ∧ (∀x. x ∈ FDOM f1 ⇒ R (f1 ' x) (f2 ' x))`
+
+val fmap_rel_FUPDATE_same = store_thm(
+"fmap_rel_FUPDATE_same",
+``fmap_rel R f1 f2 ∧ R v1 v2 ⇒ fmap_rel R (f1 |+ (k,v1)) (f2 |+ (k,v2))``,
+rw[fmap_rel_def,FAPPLY_FUPDATE_THM] >> rw[])
+
+val fmap_rel_FUPDATE_LIST_same = store_thm(
+"fmap_rel_FUPDATE_LIST_same",
+``∀R ls1 ls2 f1 f2.
+  fmap_rel R f1 f2 ∧ (MAP FST ls1 = MAP FST ls2) ∧ (LIST_REL R (MAP SND ls1) (MAP SND ls2))
+  ⇒ fmap_rel R (f1 |++ ls1) (f2 |++ ls2)``,
+gen_tac >>
+Induct >> Cases >> rw[FUPDATE_LIST_THM,LIST_REL_CONS1] >>
+Cases_on `ls2` >> fs[FUPDATE_LIST_THM] >>
+first_x_assum match_mp_tac >> fs[] >> rw[] >>
+qmatch_assum_rename_tac `R a (SND b)`[] >>
+Cases_on `b` >> fs[] >>
+rw[fmap_rel_FUPDATE_same])
+
+val fmap_rel_FEMPTY = store_thm(
+"fmap_rel_FEMPTY",
+``fmap_rel R FEMPTY FEMPTY``,
+rw[fmap_rel_def])
+val _ = export_rewrites["fmap_rel_FEMPTY"]
+
+val fmap_rel_refl = store_thm(
+"fmap_rel_refl",
+``(∀x. R x x) ⇒ fmap_rel R x x``,
+rw[fmap_rel_def])
+val _ = export_rewrites["fmap_rel_refl"]
+
+val fmap_rel_FUNION_rels = store_thm(
+"fmap_rel_FUNION_rels",
+``fmap_rel R f1 f2 ∧ fmap_rel R f3 f4 ⇒ fmap_rel R (f1 ⊌ f3) (f2 ⊌ f4)``,
+rw[fmap_rel_def,FUNION_DEF] >> rw[])
+
+val LEAST_BOUND = store_thm(
+"LEAST_BOUND",
+``∀P n. P n ⇒ ($LEAST P) ≤ n ∧ ($LEAST P = $LEAST (λm. P m ∧ m ≤ n))``,
+rpt gen_tac >>
+strip_tac >>
+conj_tac >- (
+  spose_not_then strip_assume_tac >>
+  `n < $LEAST P` by DECIDE_TAC >>
+  PROVE_TAC[whileTheory.LESS_LEAST] ) >>
+qmatch_abbrev_tac `X = Y` >>
+qunabbrev_tac`Y` >>
+numLib.LEAST_ELIM_TAC >>
+rw[Abbr`X`] >- (
+  qexists_tac `n` >> rw[] ) >>
+numLib.LEAST_ELIM_TAC >>
+rw[] >- PROVE_TAC[] >>
+qmatch_rename_tac `a = b`[] >>
+Cases_on`b < a` >- PROVE_TAC[] >>
+Cases_on`a < b` >- (
+  res_tac >> DECIDE_TAC ) >>
+DECIDE_TAC)
+
+val ALOOKUP_ALL_DISTINCT_MEM = store_thm(
+"ALOOKUP_ALL_DISTINCT_MEM",
+``ALL_DISTINCT (MAP FST al) ∧ MEM (k,v) al ⇒
+  (ALOOKUP al k = SOME v)``,
+rw[ALOOKUP_LEAST_EL] >- (
+  rw[MEM_MAP,pairTheory.EXISTS_PROD] >>
+  PROVE_TAC[]) >>
+fs[MEM_EL] >>
+pop_assum (assume_tac o SYM) >>
+qho_match_abbrev_tac `EL ($LEAST P) (MAP SND al) = v` >>
+`P n` by (
+  unabbrev_all_tac >> rw[EL_MAP] ) >>
+qspecl_then [`P`,`n`] mp_tac LEAST_BOUND >> rw[] >>
+numLib.LEAST_ELIM_TAC >>
+conj_tac >- (
+  qexists_tac `n` >> rw[] ) >>
+rw[] >>
+qmatch_rename_tac `EL m (MAP SND al) = v`[] >>
+`m < LENGTH al` by DECIDE_TAC >>
+fs[EL_ALL_DISTINCT_EL_EQ] >>
+unabbrev_all_tac >> fs[] >>
+`m = n` by PROVE_TAC[] >>
+fs[EL_MAP])
+
+val FUPDATE_LIST_ALL_DISTINCT_APPLY_MEM = store_thm(
+"FUPDATE_LIST_ALL_DISTINCT_APPLY_MEM",
+``!P ls k v fm. ALL_DISTINCT (MAP FST ls) ∧
+  MEM (k,v) ls ∧
+  P v ⇒
+  P ((fm |++ ls) ' k)``,
+rw[] >>
+ho_match_mp_tac FUPDATE_LIST_APPLY_HO_THM >>
+disj1_tac >>
+fs[EL_ALL_DISTINCT_EL_EQ,MEM_EL] >>
+qpat_assum `(k,v) = X` (assume_tac o SYM) >>
+qexists_tac `n` >> rw[EL_MAP] >>
+first_x_assum (qspecl_then [`n`,`m`] mp_tac) >>
+rw[EL_MAP] >> spose_not_then strip_assume_tac >>
+rw[] >> fs[])
+
+val DRESTRICT_FDOM = store_thm(
+"DRESTRICT_FDOM",
+``DRESTRICT fm (FDOM fm) = fm``,
+SRW_TAC[][GSYM fmap_EQ_THM,DRESTRICT_DEF])
+
+val FRANGE_DRESTRICT_SUBSET = store_thm(
+"FRANGE_DRESTRICT_SUBSET",
+``FRANGE (DRESTRICT fm s) ⊆ FRANGE fm``,
+SRW_TAC[][FRANGE_DEF,SUBSET_DEF,DRESTRICT_DEF] THEN
+SRW_TAC[][] THEN PROVE_TAC[])
+
+val DROP_NIL = store_thm(
+"DROP_NIL",
+``∀ls n. (DROP n ls = []) = (n ≥ LENGTH ls)``,
+Induct >> rw[] >>
+srw_tac[ARITH_ss][])
+
+val EVERY2_MAP = store_thm("EVERY2_MAP",
+  ``(EVERY2 P (MAP f l1) l2 = EVERY2 (λx y. P (f x) y) l1 l2) ∧
+    (EVERY2 Q l1 (MAP g l2) = EVERY2 (λx y. Q x (g y)) l1 l2)``,
+  rw[EVERY2_EVERY] >>
+  Cases_on `LENGTH l1 = LENGTH l2` >> fs[] >>
+  rw[ZIP_MAP,EVERY_MEM,MEM_MAP] >>
+  srw_tac[DNF_ss][pairTheory.FORALL_PROD] >>
+  PROVE_TAC[])
+
+val FUNION_IDEMPOT = store_thm("FUNION_IDEMPOT",
+  ``fm ⊌ fm = fm``,
+  SRW_TAC[][GSYM fmap_EQ_THM,FUNION_DEF])
+
+val FUNION_alist_to_fmap = store_thm("FUNION_alist_to_fmap",
+  ``∀ls fm. alist_to_fmap ls ⊌ fm = fm |++ (REVERSE ls)``,
+  Induct >- rw[FUNION_FEMPTY_1,FUPDATE_LIST] >>
+  qx_gen_tac `p` >> PairCases_on `p` >>
+  rw[FUPDATE_LIST_THM,alist_to_fmap_thm,FUPDATE_LIST_APPEND] >>
+  rw[FUNION_FUPDATE_1])
+
+val FUPDATE_LIST_ALL_DISTINCT_REVERSE = store_thm("FUPDATE_LIST_ALL_DISTINCT_REVERSE",
+  ``∀ls. ALL_DISTINCT (MAP FST ls) ⇒ ∀fm. fm |++ (REVERSE ls) = fm |++ ls``,
+  Induct >- rw[] >>
+  qx_gen_tac `p` >> PairCases_on `p` >>
+  rw[FUPDATE_LIST_APPEND,FUPDATE_LIST_THM] >>
+  fs[] >>
+  rw[FUPDATE_FUPDATE_LIST_COMMUTES])
+
+val _ = export_theory()
